<?xml version="1.0"?>
<rdf:RDF xmlns="http://www.semanticweb.org/CODIT/"
     xml:base="http://www.semanticweb.org/CODIT/"
     xmlns:dc="http://purl.org/dc/elements/1.1/"
     xmlns:owl="http://www.w3.org/2002/07/owl#"
     xmlns:rdf="http://www.w3.org/1999/02/22-rdf-syntax-ns#"
     xmlns:xml="http://www.w3.org/XML/1998/namespace"
     xmlns:xsd="http://www.w3.org/2001/XMLSchema#"
     xmlns:rdfs="http://www.w3.org/2000/01/rdf-schema#"
     xmlns:skos="http://www.w3.org/2004/02/skos/core#"
     xmlns:terms="http://purl.org/dc/terms/"
     xmlns:OntologyDITools="http://www.semanticweb.org/CODIT#">
    <owl:Ontology rdf:about="http://www.semanticweb.org/CODIT">
        <owl:imports rdf:resource="http://purl.org/dc/elements/1.1/"/>
        <dc:rights xml:lang="en">https://creativecommons.org/licenses/by/4.0/</dc:rights>
    </owl:Ontology>
    


    <!-- 
    ///////////////////////////////////////////////////////////////////////////////////////
    //
    // Annotation properties
    //
    ///////////////////////////////////////////////////////////////////////////////////////
     -->

    


    <!-- http://purl.org/dc/elements/1.1/rights -->

    <owl:AnnotationProperty rdf:about="http://purl.org/dc/elements/1.1/rights"/>
    


    <!-- http://www.w3.org/2002/07/owl#deprecated -->

    <rdf:Description rdf:about="http://www.w3.org/2002/07/owl#deprecated">
        <rdfs:comment xml:lang="en">The types of keys used for data interlinking typically include: primary key, composite key, almost key, etc.</rdfs:comment>
        <rdfs:label xml:lang="en">Form of the key</rdfs:label>
        <rdfs:domain rdf:resource="http://www.semanticweb.org/CODIT#keyBasedMethod"/>
    </rdf:Description>
    


    <!-- 
    ///////////////////////////////////////////////////////////////////////////////////////
    //
    // Object Properties
    //
    ///////////////////////////////////////////////////////////////////////////////////////
     -->

    


    <!-- http://www.semanticweb.org/CODIT#acceptsData -->

    <owl:ObjectProperty rdf:about="http://www.semanticweb.org/CODIT#acceptsData">
        <rdfs:subPropertyOf rdf:resource="http://www.w3.org/2002/07/owl#topObjectProperty"/>
        <rdfs:domain rdf:resource="http://www.semanticweb.org/CODIT#LinkingTool"/>
        <rdfs:range rdf:resource="http://www.semanticweb.org/CODIT#InputData"/>
        <rdfs:comment xml:lang="en">Describes the data formats and types the tool can accept.</rdfs:comment>
        <rdfs:label xml:lang="en">Accepts data</rdfs:label>
    </owl:ObjectProperty>
    


    <!-- http://www.semanticweb.org/CODIT#appliedIn -->

    <owl:ObjectProperty rdf:about="http://www.semanticweb.org/CODIT#appliedIn">
        <rdfs:subPropertyOf rdf:resource="http://www.w3.org/2002/07/owl#topObjectProperty"/>
        <rdfs:domain rdf:resource="http://www.semanticweb.org/CODIT#LinkingTool"/>
        <rdfs:range rdf:resource="http://www.semanticweb.org/CODIT#LinkingProbemType"/>
        <rdfs:comment xml:lang="en">Links the tool to the domains (e.g., healthcare, e-commerce) where it is applied.</rdfs:comment>
        <rdfs:label xml:lang="en">Applied in</rdfs:label>
    </owl:ObjectProperty>
    


    <!-- http://www.semanticweb.org/CODIT#evaluatedBy -->

    <owl:ObjectProperty rdf:about="http://www.semanticweb.org/CODIT#evaluatedBy">
        <rdfs:subPropertyOf rdf:resource="http://www.w3.org/2002/07/owl#topObjectProperty"/>
        <rdfs:domain rdf:resource="http://www.semanticweb.org/CODIT#LinkingTool"/>
        <rdfs:range rdf:resource="http://www.semanticweb.org/CODIT#PerformanceMetric"/>
        <rdfs:comment xml:lang="en">Relates the tool to the metrics by which it is evaluated (e.g., precision, recall).</rdfs:comment>
        <rdfs:label xml:lang="en">Evaluated by</rdfs:label>
    </owl:ObjectProperty>
    


    <!-- http://www.semanticweb.org/CODIT#hasDependency -->

    <owl:ObjectProperty rdf:about="http://www.semanticweb.org/CODIT#hasDependency">
        <rdfs:subPropertyOf rdf:resource="http://www.w3.org/2002/07/owl#topObjectProperty"/>
        <rdfs:domain rdf:resource="http://www.semanticweb.org/CODIT#LinkingTool"/>
        <rdfs:range rdf:resource="http://www.semanticweb.org/CODIT#Dependency"/>
        <rdfs:comment xml:lang="en">Describes any external resources necessary for the tool to function.</rdfs:comment>
        <rdfs:label xml:lang="en">Has dependency</rdfs:label>
    </owl:ObjectProperty>
    


    <!-- http://www.semanticweb.org/CODIT#hasFeature -->

    <owl:ObjectProperty rdf:about="http://www.semanticweb.org/CODIT#hasFeature">
        <rdfs:subPropertyOf rdf:resource="http://www.w3.org/2002/07/owl#topObjectProperty"/>
        <rdfs:domain rdf:resource="http://www.semanticweb.org/CODIT#LinkingTool"/>
        <rdfs:range rdf:resource="http://www.semanticweb.org/CODIT#Feature"/>
        <rdfs:comment xml:lang="en">Associates the tool with specific features that it provides.</rdfs:comment>
        <rdfs:label xml:lang="en">Has feature</rdfs:label>
    </owl:ObjectProperty>
    


    <!-- http://www.semanticweb.org/CODIT#producesOutput -->

    <owl:ObjectProperty rdf:about="http://www.semanticweb.org/CODIT#producesOutput">
        <rdfs:subPropertyOf rdf:resource="http://www.w3.org/2002/07/owl#topObjectProperty"/>
        <rdfs:domain rdf:resource="http://www.semanticweb.org/CODIT#LinkingTool"/>
        <rdfs:range rdf:resource="http://www.semanticweb.org/CODIT#OutputData"/>
        <rdfs:comment xml:lang="en">Links the tool to the resulting output format (e.g., RDF, JSON).</rdfs:comment>
        <rdfs:label xml:lang="en">Produces output</rdfs:label>
    </owl:ObjectProperty>
    


    <!-- http://www.semanticweb.org/CODIT#suitedFor -->

    <owl:ObjectProperty rdf:about="http://www.semanticweb.org/CODIT#suitedFor">
        <rdfs:subPropertyOf rdf:resource="http://www.w3.org/2002/07/owl#topObjectProperty"/>
        <rdfs:domain rdf:resource="http://www.semanticweb.org/CODIT#LinkingTool"/>
        <rdfs:range rdf:resource="http://www.semanticweb.org/CODIT#LinkingProbemType"/>
        <rdfs:comment xml:lang="en">Connects the tool to tasks it can handle (e.g., large-scale data, different-format data).</rdfs:comment>
        <rdfs:label xml:lang="en">Suited for</rdfs:label>
    </owl:ObjectProperty>
    


    <!-- http://www.semanticweb.org/CODIT#usesAlgorithm -->

    <owl:ObjectProperty rdf:about="http://www.semanticweb.org/CODIT#usesAlgorithm">
        <rdfs:subPropertyOf rdf:resource="http://www.w3.org/2002/07/owl#topObjectProperty"/>
        <rdfs:domain rdf:resource="http://www.semanticweb.org/CODIT#Training"/>
        <rdfs:range rdf:resource="http://www.semanticweb.org/CODIT#TrainingAlgorithm"/>
        <rdfs:comment xml:lang="en">Associate the tool with the training algorithm it uses.</rdfs:comment>
        <rdfs:label xml:lang="en">Uses algorithm</rdfs:label>
    </owl:ObjectProperty>
    


    <!-- http://www.semanticweb.org/CODIT#usesData -->

    <owl:ObjectProperty rdf:about="http://www.semanticweb.org/CODIT#usesData">
        <rdfs:subPropertyOf rdf:resource="http://www.w3.org/2002/07/owl#topObjectProperty"/>
        <rdfs:domain rdf:resource="http://www.semanticweb.org/CODIT#Training"/>
        <rdfs:range rdf:resource="http://www.semanticweb.org/CODIT#TrainingData"/>
        <rdfs:comment xml:lang="en">Links the tool with the training data it uses.</rdfs:comment>
        <rdfs:label xml:lang="en">Uses data</rdfs:label>
    </owl:ObjectProperty>
    


    <!-- http://www.semanticweb.org/CODIT#usesTechnique -->

    <owl:ObjectProperty rdf:about="http://www.semanticweb.org/CODIT#usesTechnique">
        <rdfs:subPropertyOf rdf:resource="http://www.w3.org/2002/07/owl#topObjectProperty"/>
        <rdfs:domain rdf:resource="http://www.semanticweb.org/CODIT#LinkingTool"/>
        <rdfs:range rdf:resource="http://www.semanticweb.org/CODIT#LinkingTechnique"/>
        <rdfs:comment xml:lang="en">Links the tool to the techniques it implements.</rdfs:comment>
        <rdfs:label xml:lang="en">Uses technique</rdfs:label>
    </owl:ObjectProperty>
    


    <!-- 
    ///////////////////////////////////////////////////////////////////////////////////////
    //
    // Data properties
    //
    ///////////////////////////////////////////////////////////////////////////////////////
     -->

    


    <!-- http://purl.org/dc/elements/1.1/format -->

    <owl:DatatypeProperty rdf:about="http://purl.org/dc/elements/1.1/format"/>
    


    <!-- http://purl.org/dc/elements/1.1/hasVersion -->

    <owl:DatatypeProperty rdf:about="http://purl.org/dc/elements/1.1/hasVersion">
        <rdfs:subPropertyOf rdf:resource="http://www.w3.org/2002/07/owl#topDataProperty"/>
    </owl:DatatypeProperty>
    


    <!-- http://purl.org/dc/elements/1.1/source -->

    <owl:DatatypeProperty rdf:about="http://purl.org/dc/elements/1.1/source"/>
    


    <!-- http://www.semanticweb.org/CODIT#AxiomGenCriteria -->

    <owl:DatatypeProperty rdf:about="http://www.semanticweb.org/CODIT#AxiomGenCriteria">
        <rdfs:subPropertyOf rdf:resource="http://www.w3.org/2002/07/owl#topDataProperty"/>
        <rdfs:domain rdf:resource="http://www.semanticweb.org/CODIT#Symbolic"/>
        <rdfs:range rdf:resource="http://www.w3.org/2001/XMLSchema#string"/>
        <rdfs:comment xml:lang="en">The criteria used to generate axiom i.e., rules of keys.</rdfs:comment>
        <rdfs:label xml:lang="en">Axiom Generation Criteria</rdfs:label>
    </owl:DatatypeProperty>
    


    <!-- http://www.semanticweb.org/CODIT#LinkGenCriteria -->

    <owl:DatatypeProperty rdf:about="http://www.semanticweb.org/CODIT#LinkGenCriteria">
        <rdfs:subPropertyOf rdf:resource="http://www.w3.org/2002/07/owl#topDataProperty"/>
        <rdfs:domain rdf:resource="http://www.semanticweb.org/CODIT#NonSymbolic"/>
        <rdfs:range rdf:resource="http://www.w3.org/2001/XMLSchema#string"/>
        <rdfs:comment xml:lang="en">The fundamental reasons behined link generation.</rdfs:comment>
        <rdfs:label xml:lang="en">Link Generation Criteria</rdfs:label>
    </owl:DatatypeProperty>
    


    <!-- http://www.semanticweb.org/CODIT#category -->

    <owl:DatatypeProperty rdf:about="http://www.semanticweb.org/CODIT#category">
        <rdfs:subPropertyOf rdf:resource="http://www.w3.org/2002/07/owl#topDataProperty"/>
        <rdfs:domain>
            <owl:Class>
                <owl:unionOf rdf:parseType="Collection">
                    <rdf:Description rdf:about="http://www.semanticweb.org/CODIT#InputData"/>
                    <rdf:Description rdf:about="http://www.semanticweb.org/CODIT#OutputData"/>
                    <rdf:Description rdf:about="http://www.semanticweb.org/CODIT#TrainingData"/>
                </owl:unionOf>
            </owl:Class>
        </rdfs:domain>
        <rdfs:range rdf:resource="http://www.w3.org/2001/XMLSchema#string"/>
        <rdfs:comment xml:lang="en">The type of the data, applicable to both input and output, such as structured, semi-structured, or unstructured.&quot;</rdfs:comment>
        <rdfs:label xml:lang="en">Category</rdfs:label>
    </owl:DatatypeProperty>
    


    <!-- http://www.semanticweb.org/CODIT#configuration -->

    <owl:DatatypeProperty rdf:about="http://www.semanticweb.org/CODIT#configuration">
        <rdfs:subPropertyOf rdf:resource="http://www.w3.org/2002/07/owl#topDataProperty"/>
        <rdfs:domain rdf:resource="http://www.semanticweb.org/CODIT#LinkingTool"/>
        <rdfs:range rdf:resource="http://www.w3.org/2001/XMLSchema#string"/>
        <rdfs:comment xml:lang="en">Specifies the parameters or settings required to configure the tool.</rdfs:comment>
        <rdfs:label xml:lang="en">Configuration</rdfs:label>
    </owl:DatatypeProperty>
    


    <!-- http://www.semanticweb.org/CODIT#dimensionality -->

    <owl:DatatypeProperty rdf:about="http://www.semanticweb.org/CODIT#dimensionality">
        <rdfs:subPropertyOf rdf:resource="http://www.w3.org/2002/07/owl#topDataProperty"/>
        <rdfs:domain rdf:resource="http://www.semanticweb.org/CODIT#EmbeddingBasedMethod"/>
        <rdfs:range rdf:resource="http://www.w3.org/2001/XMLSchema#string"/>
        <rdfs:comment xml:lang="en">Represents the number of dimensions in the embedding space.</rdfs:comment>
        <rdfs:label xml:lang="en">Dimensionality</rdfs:label>
    </owl:DatatypeProperty>
    


    <!-- http://www.semanticweb.org/CODIT#embeddingAlgorithm -->

    <owl:DatatypeProperty rdf:about="http://www.semanticweb.org/CODIT#embeddingAlgorithm">
        <rdfs:subPropertyOf rdf:resource="http://www.w3.org/2002/07/owl#topDataProperty"/>
        <rdfs:domain rdf:resource="http://www.semanticweb.org/CODIT#EmbeddingBasedMethod"/>
        <rdfs:range rdf:resource="http://www.w3.org/2001/XMLSchema#string"/>
        <rdfs:comment xml:lang="en">Specifies the algorithm used for generating embeddings, such as Word2Vec, BERT, or TransE.</rdfs:comment>
        <rdfs:label xml:lang="en">Embedding Algorithm</rdfs:label>
    </owl:DatatypeProperty>
    


    <!-- http://www.semanticweb.org/CODIT#fineTuning -->

    <owl:DatatypeProperty rdf:about="http://www.semanticweb.org/CODIT#fineTuning">
        <rdfs:subPropertyOf rdf:resource="http://www.w3.org/2002/07/owl#topDataProperty"/>
        <rdfs:domain rdf:resource="http://www.semanticweb.org/CODIT#LLMMethod"/>
        <rdfs:range rdf:resource="http://www.w3.org/2001/XMLSchema#string"/>
        <rdfs:comment xml:lang="en">Indicates whether the large language model has been fine-tuned on specific data for the entity matching task.</rdfs:comment>
        <rdfs:label xml:lang="en">Fine-Tuning</rdfs:label>
    </owl:DatatypeProperty>
    


    <!-- http://www.semanticweb.org/CODIT#hyper-parameters -->

    <owl:DatatypeProperty rdf:about="http://www.semanticweb.org/CODIT#hyper-parameters">
        <rdfs:subPropertyOf rdf:resource="http://www.w3.org/2002/07/owl#topDataProperty"/>
        <rdfs:domain rdf:resource="http://www.semanticweb.org/CODIT#Training"/>
        <rdfs:range rdf:resource="http://www.w3.org/2001/XMLSchema#string"/>
        <rdfs:comment xml:lang="en">The settings of the tool including the learning_rate, batch_size and other specifications that impact on the results.</rdfs:comment>
        <rdfs:label xml:lang="en">Hyper-parameters</rdfs:label>
    </owl:DatatypeProperty>
    


    <!-- http://www.semanticweb.org/CODIT#iterations -->

    <owl:DatatypeProperty rdf:about="http://www.semanticweb.org/CODIT#iterations">
        <rdfs:subPropertyOf rdf:resource="http://www.w3.org/2002/07/owl#topDataProperty"/>
        <rdfs:domain rdf:resource="http://www.semanticweb.org/CODIT#Training"/>
        <rdfs:range rdf:resource="http://www.w3.org/2001/XMLSchema#integer"/>
        <rdfs:comment xml:lang="en">Specify the number of iteration needed for training the tool.</rdfs:comment>
        <rdfs:label xml:lang="en">Number of Iterations</rdfs:label>
    </owl:DatatypeProperty>
    


    <!-- http://www.semanticweb.org/CODIT#keyForm -->

    <owl:DatatypeProperty rdf:about="http://www.semanticweb.org/CODIT#keyForm">
        <rdfs:subPropertyOf rdf:resource="http://www.w3.org/2002/07/owl#topDataProperty"/>
        <rdfs:domain rdf:resource="http://www.semanticweb.org/CODIT#keyBasedMethod"/>
        <rdfs:range rdf:resource="http://www.w3.org/2001/XMLSchema#string"/>
        <rdfs:comment xml:lang="en">Describes the criteria used to match keys, such as exact match or approximate match.</rdfs:comment>
        <rdfs:label xml:lang="en">Key form</rdfs:label>
    </owl:DatatypeProperty>
    


    <!-- http://www.semanticweb.org/CODIT#kind -->

    <owl:DatatypeProperty rdf:about="http://www.semanticweb.org/CODIT#kind">
        <rdfs:subPropertyOf rdf:resource="http://www.w3.org/2002/07/owl#topDataProperty"/>
        <rdfs:domain rdf:resource="http://www.semanticweb.org/CODIT#PerformanceMetric"/>
        <rdfs:range rdf:resource="http://www.w3.org/2001/XMLSchema#string"/>
        <rdfs:comment xml:lang="en">Describes the kind of the evaluation metric used, i.e., supervised or un-supervised.</rdfs:comment>
        <rdfs:label xml:lang="en">Kind</rdfs:label>
    </owl:DatatypeProperty>
    


    <!-- http://www.semanticweb.org/CODIT#promptDesign -->

    <owl:DatatypeProperty rdf:about="http://www.semanticweb.org/CODIT#promptDesign">
        <rdfs:subPropertyOf rdf:resource="http://www.w3.org/2002/07/owl#topDataProperty"/>
        <rdfs:domain rdf:resource="http://www.semanticweb.org/CODIT#LLMMethod"/>
        <rdfs:range rdf:resource="http://www.w3.org/2001/XMLSchema#string"/>
        <rdfs:comment xml:lang="en">Describes the structure of the prompts used to interact with the large language model, such as zero-shot or few-shot prompting.</rdfs:comment>
        <rdfs:label xml:lang="en">Prompt Design</rdfs:label>
    </owl:DatatypeProperty>
    


    <!-- http://www.semanticweb.org/CODIT#requiresTraining -->

    <owl:DatatypeProperty rdf:about="http://www.semanticweb.org/CODIT#requiresTraining">
        <rdfs:subPropertyOf rdf:resource="http://www.w3.org/2002/07/owl#topDataProperty"/>
        <rdfs:domain rdf:resource="http://www.semanticweb.org/CODIT#LinkingTool"/>
        <rdfs:range rdf:resource="http://www.w3.org/2001/XMLSchema#boolean"/>
        <rdfs:comment xml:lang="en">A boolean used to indicate wether the linking tool requires training or not.</rdfs:comment>
        <rdfs:label xml:lang="en">Requires training</rdfs:label>
    </owl:DatatypeProperty>
    


    <!-- http://www.semanticweb.org/CODIT#ruleDefinitionLanguage -->

    <owl:DatatypeProperty rdf:about="http://www.semanticweb.org/CODIT#ruleDefinitionLanguage">
        <rdfs:subPropertyOf rdf:resource="http://www.w3.org/2002/07/owl#topDataProperty"/>
        <rdfs:domain rdf:resource="http://www.semanticweb.org/CODIT#RuleBasedMethod"/>
        <rdfs:range rdf:resource="http://www.w3.org/2001/XMLSchema#string"/>
        <rdfs:comment xml:lang="en">Specifies the language or framework used to define rules, such as SPARQL or SQL.</rdfs:comment>
        <rdfs:label xml:lang="en">Rule Definition Language</rdfs:label>
    </owl:DatatypeProperty>
    


    <!-- http://www.semanticweb.org/CODIT#source -->

    <owl:DatatypeProperty rdf:about="http://www.semanticweb.org/CODIT#source">
        <rdfs:subPropertyOf rdf:resource="http://purl.org/dc/elements/1.1/source"/>
        <rdfs:domain>
            <owl:Class>
                <owl:unionOf rdf:parseType="Collection">
                    <rdf:Description rdf:about="http://www.semanticweb.org/CODIT#Dependency"/>
                    <rdf:Description rdf:about="http://www.semanticweb.org/CODIT#LinkingTool"/>
                </owl:unionOf>
            </owl:Class>
        </rdfs:domain>
        <rdfs:range rdf:resource="http://www.w3.org/2001/XMLSchema#string"/>
        <rdfs:comment xml:lang="en">Specifies the origin or URL of the developer or dependency.</rdfs:comment>
        <rdfs:label xml:lang="en">Source</rdfs:label>
    </owl:DatatypeProperty>
    


    <!-- http://www.semanticweb.org/CODIT#version -->

    <owl:DatatypeProperty rdf:about="http://www.semanticweb.org/CODIT#version">
        <rdfs:subPropertyOf rdf:resource="http://purl.org/dc/elements/1.1/hasVersion"/>
        <rdfs:domain>
            <owl:Class>
                <owl:unionOf rdf:parseType="Collection">
                    <rdf:Description rdf:about="http://www.semanticweb.org/CODIT#Dependency"/>
                    <rdf:Description rdf:about="http://www.semanticweb.org/CODIT#LinkingTool"/>
                </owl:unionOf>
            </owl:Class>
        </rdfs:domain>
        <rdfs:range rdf:resource="http://www.w3.org/2001/XMLSchema#string"/>
        <rdfs:comment xml:lang="en">Represents the specific version of the tool or the dependency.</rdfs:comment>
        <rdfs:label xml:lang="en">Version</rdfs:label>
    </owl:DatatypeProperty>
    


    <!-- 
    ///////////////////////////////////////////////////////////////////////////////////////
    //
    // Classes
    //
    ///////////////////////////////////////////////////////////////////////////////////////
     -->

    


    <!-- http://www.semanticweb.org/CODIT#ApplicationDomain -->

    <owl:Class rdf:about="http://www.semanticweb.org/CODIT#ApplicationDomain">
        <terms:description></terms:description>
        <terms:title></terms:title>
        <rdfs:comment xml:lang="en">Specifies the domain(s) in which the linking tool can be applied, such as healthcare, e-commerce, etc.</rdfs:comment>
        <rdfs:label xml:lang="en">Application Domain</rdfs:label>
    </owl:Class>
    


    <!-- http://www.semanticweb.org/CODIT#Dependency -->

    <owl:Class rdf:about="http://www.semanticweb.org/CODIT#Dependency">
        <terms:description></terms:description>
        <terms:publisher></terms:publisher>
        <terms:title></terms:title>
        <rdfs:comment xml:lang="en">Represents external libraries or resources required by a linking tool.</rdfs:comment>
        <rdfs:label xml:lang="en">Dependency</rdfs:label>
    </owl:Class>
    


    <!-- http://www.semanticweb.org/CODIT#EmbeddingBasedMethod -->

    <owl:Class rdf:about="http://www.semanticweb.org/CODIT#EmbeddingBasedMethod">
        <rdfs:subClassOf rdf:resource="http://www.semanticweb.org/CODIT#NonSymbolic"/>
        <owl:disjointWith rdf:resource="http://www.semanticweb.org/CODIT#RuleBasedMethod"/>
        <rdfs:comment xml:lang="en">A method that uses embeddings (vector representations) for linking.</rdfs:comment>
        <rdfs:label xml:lang="en">Embedding Based Method</rdfs:label>
    </owl:Class>
    


    <!-- http://www.semanticweb.org/CODIT#Feature -->

    <owl:Class rdf:about="http://www.semanticweb.org/CODIT#Feature">
        <terms:description></terms:description>
        <terms:title></terms:title>
        <rdfs:comment xml:lang="en">Describes specific capabilities or functionalities of a linking tool.</rdfs:comment>
        <rdfs:label xml:lang="en">Feature</rdfs:label>
    </owl:Class>
    


    <!-- http://www.semanticweb.org/CODIT#InputData -->

    <owl:Class rdf:about="http://www.semanticweb.org/CODIT#InputData">
        <terms:description></terms:description>
        <rdfs:comment xml:lang="en">Represents the input data structure and format that a linking tool can process.</rdfs:comment>
        <rdfs:label xml:lang="en">Input Data</rdfs:label>
    </owl:Class>
    


    <!-- http://www.semanticweb.org/CODIT#LLMMethod -->

    <owl:Class rdf:about="http://www.semanticweb.org/CODIT#LLMMethod">
        <rdfs:subClassOf rdf:resource="http://www.semanticweb.org/CODIT#NonSymbolic"/>
        <rdfs:comment xml:lang="en">A linking technique that leverages large language models (LLMs) for entity matching.</rdfs:comment>
        <rdfs:label xml:lang="en">LLM Method</rdfs:label>
    </owl:Class>
    


    <!-- http://www.semanticweb.org/CODIT#LinkingProbemType -->

    <owl:Class rdf:about="http://www.semanticweb.org/CODIT#LinkingProbemType">
        <terms:description></terms:description>
        <terms:title></terms:title>
        <rdfs:comment xml:lang="en">Represents a linking problem type that a linking tool is suited to perform, such as large scale data or datasets with different schemas.</rdfs:comment>
        <rdfs:label xml:lang="en">Linking Problem Type (LPT)</rdfs:label>
    </owl:Class>
    


    <!-- http://www.semanticweb.org/CODIT#LinkingTechnique -->

    <owl:Class rdf:about="http://www.semanticweb.org/CODIT#LinkingTechnique">
        <terms:description></terms:description>
        <terms:title></terms:title>
        <rdfs:comment xml:lang="en">Represents the methods and criteria used for linking entities across datasets. Includes various techniques like Rule-Based, String Similarity, and Machine Learning methods.</rdfs:comment>
        <rdfs:label xml:lang="en">Linking Technique</rdfs:label>
    </owl:Class>
    


    <!-- http://www.semanticweb.org/CODIT#LinkingTool -->

    <owl:Class rdf:about="http://www.semanticweb.org/CODIT#LinkingTool">
        <terms:description></terms:description>
        <terms:publisher></terms:publisher>
        <terms:title></terms:title>
        <rdfs:comment xml:lang="en">Represents a data interlinking tool used for linking entities across different datasets or knowledge graphs.</rdfs:comment>
        <rdfs:label xml:lang="en">Linking Tool</rdfs:label>
    </owl:Class>
    


    <!-- http://www.semanticweb.org/CODIT#NonSymbolic -->

    <owl:Class rdf:about="http://www.semanticweb.org/CODIT#NonSymbolic">
        <rdfs:subClassOf rdf:resource="http://www.semanticweb.org/CODIT#LinkingTechnique"/>
        <rdfs:comment xml:lang="en">Employ machine learning to discover latent patterns for entity matching, excelling in scalability but often lacking interpretability.</rdfs:comment>
        <rdfs:label xml:lang="en">Non-Symbolic</rdfs:label>
    </owl:Class>
    


    <!-- http://www.semanticweb.org/CODIT#OutputData -->

    <owl:Class rdf:about="http://www.semanticweb.org/CODIT#OutputData">
        <terms:description></terms:description>
        <rdfs:comment xml:lang="en">Describes the characteristics of the output data generated by a linking tool.</rdfs:comment>
        <rdfs:label xml:lang="en">Output Data</rdfs:label>
    </owl:Class>
    


    <!-- http://www.semanticweb.org/CODIT#PerformanceMetric -->

    <owl:Class rdf:about="http://www.semanticweb.org/CODIT#PerformanceMetric">
        <terms:description></terms:description>
        <terms:title></terms:title>
        <rdfs:comment xml:lang="en">Specifies the evaluation metrics used to assess the performance of a linking tool.</rdfs:comment>
        <rdfs:label xml:lang="en">Performance Metric</rdfs:label>
    </owl:Class>
    


    <!-- http://www.semanticweb.org/CODIT#RuleBasedMethod -->

    <owl:Class rdf:about="http://www.semanticweb.org/CODIT#RuleBasedMethod">
        <rdfs:subClassOf rdf:resource="http://www.semanticweb.org/CODIT#Symbolic"/>
        <rdfs:comment xml:lang="en">A technique based on predefined rules to link entities.</rdfs:comment>
        <rdfs:label xml:lang="en">Rule Based Method</rdfs:label>
    </owl:Class>
    


    <!-- http://www.semanticweb.org/CODIT#Symbolic -->

    <owl:Class rdf:about="http://www.semanticweb.org/CODIT#Symbolic">
        <rdfs:subClassOf rdf:resource="http://www.semanticweb.org/CODIT#LinkingTechnique"/>
        <rdfs:comment xml:lang="en">Use predefined rules, logical reasoning, or schema alignment to match entities, offering high explainability but limited scalability.</rdfs:comment>
        <rdfs:label xml:lang="en">Symbolic</rdfs:label>
    </owl:Class>
    


    <!-- http://www.semanticweb.org/CODIT#Training -->

    <owl:Class rdf:about="http://www.semanticweb.org/CODIT#Training">
        <rdfs:comment xml:lang="en">Represents the training configuration for machine learning models used in data linking.</rdfs:comment>
        <rdfs:label xml:lang="en">Training</rdfs:label>
    </owl:Class>
    


    <!-- http://www.semanticweb.org/CODIT#TrainingAlgorithm -->

    <owl:Class rdf:about="http://www.semanticweb.org/CODIT#TrainingAlgorithm">
        <terms:description></terms:description>
        <terms:title></terms:title>
        <rdfs:comment xml:lang="en">The algorithm used for training the tool.</rdfs:comment>
        <rdfs:label xml:lang="en">Training Algorithm</rdfs:label>
    </owl:Class>
    


    <!-- http://www.semanticweb.org/CODIT#TrainingData -->

    <owl:Class rdf:about="http://www.semanticweb.org/CODIT#TrainingData">
        <terms:description></terms:description>
        <rdfs:comment xml:lang="en">Describes the data used for training the linking tool.</rdfs:comment>
        <rdfs:label xml:lang="en">Training Data</rdfs:label>
    </owl:Class>
    


    <!-- http://www.semanticweb.org/CODIT#keyBasedMethod -->

    <owl:Class rdf:about="http://www.semanticweb.org/CODIT#keyBasedMethod">
        <rdfs:subClassOf rdf:resource="http://www.semanticweb.org/CODIT#Symbolic"/>
        <rdfs:comment xml:lang="en">A method that aims at generating keys and using them for EM.</rdfs:comment>
        <rdfs:label xml:lang="en">Key Based Method</rdfs:label>
    </owl:Class>
</rdf:RDF>



<!-- Generated by the OWL API (version 4.5.29.2024-05-13T12:11:03Z) https://github.com/owlcs/owlapi -->
